Correctness.v
@@ -8,7 +8,7 @@ Add LoadPath ".".
 
 Require Import SysF.
 
-Lemma beq_typ_correct : forall t1 t2 : typ, beq_typ t1 t2 = true -> t1 = t2.
+Lemma beq_typ_correct : forall t1 t2 : typ, beq_typ t1 t2 = true -> t1 = t2. 
   induction t1.
   - intros.
     destruct t2; [ auto using beq_nat_eq | inversion H .. ].
@@ -49,8 +49,8 @@ Theorem leq_correct : forall m n : nat, leq m n = true -> m <= n.
 Qed.
 
 (* This is actually cumulativity *)
-Lemma kinding_ind_sub : forall (e : env) (t : typ) (k : kind),
-                          kinding_ind e t k -> forall k', k <= k' -> kinding_ind e t k'.
+Lemma kinding_sub : forall (e : env) (t : typ) (k : kind),
+                          kinding e t k -> forall k', k <= k' -> kinding e t k'.
   do 4 intro.
   induction H.
   - intros.
@@ -71,12 +71,14 @@ Lemma kinding_ind_sub : forall (e : env) (t : typ) (k : kind),
     apply k_tarr; [ eauto using le_trans .. ]. (* TODO just eauto using k_tarr, le_trans doesn't work *)
 Qed.
 
+Definition cumulativity := kinding_sub.
+
 
 (* TODO simplified the equivalences to implications so this plays nice with eauto *)
 Lemma bwf_typ_correct : forall t : typ, forall e : env, bwf_typ e t = true -> wf_typ e t.
   induction t.
   - intro. simpl.
-    destruct (get_kind e n); [ intuition .. ].
+    destruct (get_kind e n); [ intuition .. ]. discriminate.
   - intros.
     (* TODO this looks like it could be shorter, but eauto doesn't work *)
     apply andb_true_iff in H.
@@ -97,7 +99,9 @@ Lemma bwf_env_correct : forall e : env, bwf_env e = true -> wf_env e.
   - apply IHe.
 Qed.
 
-Theorem kind_of_correct (t : typ) : forall (e : env) (k : kind), kind_of e t = Some k -> kinding_ind e t k.
+Theorem kind_of_correct (t : typ) : 
+  forall (e : env) (k : kind), 
+    kind_of e t = Some k -> kinding e t k.
   induction t.
   - intros. simpl in H.
     remember (bwf_env e).
@@ -115,110 +119,9 @@ Theorem kind_of_correct (t : typ) : forall (e : env) (k : kind), kind_of e t = S
     + inversion H.
 Qed. 
 
-(*
-Lemma typing_uniq :
-  forall t : term, forall e : env, forall ty1 ty2 : typ,
-    typing e t ty1 -> typing e t ty2 -> ty1 = ty2.
-  intro.
-  induction t.
-  - intros. simpl.
-    unfold typing in H, H0.
-    destruct (get_typ e n).
-    + destruct H. destruct H0.
-      apply eq_sym in H1.
-      apply (eq_trans H2) in H1.
-      auto.
-    + inversion H.
-  - intros.
-    destruct ty1.
-    + inversion H.
-    + simpl in H0.
-      destruct ty2.
-      * inversion H0.
-      * destruct H. destruct H0.
-        apply eq_sym in H0. apply (eq_trans H) in H0.
-        apply (IHt (evar ty1_1 e) ty1_2 ty2_2) in H1.
-        congruence.
-        rewrite -> H0.
-        apply H2.
-      * inversion H0.
-    + inversion H.
-  - intros.
-      destruct H. destruct H0.
-      destruct H. destruct H0.
-      apply (IHt1 e (tarr x ty1) (tarr x ty2)) in H.
-      injection H. trivial.
-      apply (IHt2 e x x0) in H1.
-      rewrite -> H1. apply H0.
-      apply H2.
-  - intros.
-    simpl in H. simpl in H0.
-    destruct ty1.
-    + inversion H.
-    + inversion H.
-    + destruct ty2.
-      * inversion H0.
-      * inversion H0.
-      * destruct H. destruct H0.
-        apply (IHt (etvar k e) ty1 ty2) in H1.
-        congruence.
-        apply H2.
-  -  intros.
-     simpl in H. simpl in H0.
-     do 3 destruct H, H0.
-     destruct H1, H2.
-     apply (IHt e (tall x x1) (tall x0 x2)) in H.
-     injection H. intros.
-     rewrite H3. rewrite H4.
-     congruence.
-     apply H0.
-Qed. 
-
-Lemma kind_of_minimal : forall t : typ, forall e : env, forall k : kind,
-                          match kind_of e t with
-                            | Some k' => kinding e t k -> k' <= k
-                            | None => True
-                          end.
-  induction t.
-  - intros.
-    simpl.
-    remember (bwf_env e) as wfenv.
-    remember (get_kind e n) as envkind.
-    destruct wfenv.
-    + destruct envkind.
-      * intros. destruct H. trivial.
-      * trivial.
-    + trivial.
-  - intros.
-    simpl.
-    specialize (IHt1 e). specialize (IHt2 e).
-    remember (kind_of e t1) as kind_t1 in IHt1 |- *.
-    remember (kind_of e t2) as kind_t2 in IHt2 |- *.
-    destruct kind_t1.
-    + destruct kind_t2.
-      * intro.
-        do 3 destruct H. destruct H0. apply IHt1 in H0. apply IHt2 in H1.
-        apply (max_case k0 k1 (fun x => x <= k)).
-        assert (x <= max x x0). auto with arith. rewrite -> H in H2. omega.
-        assert (x0 <= max x x0). auto with arith. rewrite -> H in H2. omega.
-      * trivial.
-    + trivial.
-  - intros. simpl.
-    specialize (IHt (etvar k e)).
-    remember (kind_of (etvar k e) t) as kind_e in IHt |- *.
-    destruct kind_e.
-    + intros. do 2 destruct H.
-      apply IHt in H.
-      rewrite -> H0.
-      apply le_n_S.
-      apply (max_case k k1 (fun n => n <= max x k)).
-      apply le_max_r.
-      assert (x <= max x k). apply le_max_l.
-      omega.
-    + trivial.
-Qed. *)
-          
-Theorem type_of_correct (t : term) : forall (e : env) (T : typ), type_of e t = Some T -> typing_ind e t T.
+Theorem type_of_correct (t : term) : 
+  forall (e : env) (T : typ), 
+    type_of e t = Some T -> typing e t T.
   induction t.
   - intros. simpl in H.
     destruct (bwf_env e) eqn:env_is_bwf.
@@ -226,7 +129,9 @@ Theorem type_of_correct (t : term) : forall (e : env) (T : typ), type_of e t = S
     + inversion H.
   - intros. simpl in H.
     destruct (type_of (evar t e) t0) eqn:type_of_body.
-    + inversion H. auto using t_abs.
+    + remember (bwf_typ e t). destruct b.
+      * inversion H. apply t_abs. apply bwf_typ_correct. auto. apply IHt, type_of_body.
+      * discriminate.
     + inversion H.
   - intros. simpl in H.
     destruct (type_of e t1) eqn:type_of_fn.
@@ -252,7 +157,7 @@ Theorem type_of_correct (t : term) : forall (e : env) (T : typ), type_of e t = S
       * destruct (kind_of e t0) eqn:kind_of_arg.
         { destruct (leq k0 k) eqn:k0_leq_k.
           { inversion H. eapply t_app_t. eauto.
-            eauto using kind_of_correct, leq_correct, kinding_ind_sub, t_app_t. }
+            eauto using kind_of_correct, leq_correct, kinding_sub, t_app_t. }
           { inversion H. } }
         { inversion H. }
     + inversion H.
